Veil/Model/TransitionSystem.lean
@@ -1,48 +1,54 @@
+import Aesop
 
-class RelationalTransitionSystem (ρ : Type) (σ : Type) where
+class RelationalTransitionSystem (ρ : Type) (σ : Type) (l : outParam Type) where
   /-- The set of acceptable background theories -/
   assumptions : ρ → Prop
   /-- The set of initial states, indexed by background theory they
   operate in -/
   init : ρ → σ → Prop
   /-- The transition relation -/
-  next : ρ → σ -> σ -> Prop
+  nextLab : ρ → σ → l → σ → Prop
   safe : ρ → σ → Prop
   inv : ρ → σ → Prop
 
   initSatisfiesAssumptions : ∀ (r : ρ) (s : σ), init r s → assumptions r
 
+def RelationalTransitionSystem.next [RelationalTransitionSystem ρ σ l] (r : ρ) (s : σ) (s' : σ) : Prop :=
+  ∃ l, nextLab r s l s'
+
 namespace RelationalTransitionSystem
 open RelationalTransitionSystem
 
+
 /-- All states in the invariant are safe. -/
-def invSafe [RelationalTransitionSystem ρ σ] :=
-  ∀ (r : ρ) (s : σ), @assumptions ρ σ _ r -> inv r s -> safe r s
+def invSafe [RelationalTransitionSystem ρ σ l] :=
+  ∀ (r : ρ) (s : σ), @assumptions ρ σ l _ r -> inv r s -> safe r s
 
 /-- The set of initial states are in the invariant. -/
-def invInit [RelationalTransitionSystem ρ σ] (p : ρ → σ → Prop) :=
-  ∀ (r : ρ) (s : σ), @assumptions ρ σ _ r -> init r s -> p r s
+def invInit [RelationalTransitionSystem ρ σ l] (p : ρ → σ → Prop) :=
+  ∀ (r : ρ) (s : σ), @assumptions ρ σ l _ r -> init r s -> p r s
 
 /-- The invariant is preserved by transition. -/
-def invConsecution [RelationalTransitionSystem ρ σ] (p : ρ → σ → Prop) :=
-  ∀ (r : ρ) (s1 s2 : σ), @assumptions ρ σ _ r -> p r s1 -> next r s1 s2 -> p r s2
+def invConsecution [RelationalTransitionSystem ρ σ l] (p : ρ → σ → Prop) :=
+  ∀ (r : ρ) (s1 s2 : σ), @assumptions ρ σ l _ r -> p r s1 -> next r s1 s2 -> p r s2
 
 /-- The invariant is inductive. -/
-def isInductive [sys: RelationalTransitionSystem ρ σ] (p : ρ → σ → Prop) :=
-  @invInit ρ σ sys p ∧ @invConsecution ρ σ sys p
+def isInductive [sys: RelationalTransitionSystem ρ σ l] (p : ρ → σ → Prop) :=
+  @invInit ρ σ l sys p ∧ @invConsecution ρ σ l sys p
 
 /-- Reachability relation, indexed by background theory -/
-inductive reachable [sys : RelationalTransitionSystem ρ σ] (r : ρ) : σ → Prop where
+@[aesop safe constructors]
+inductive reachable [sys : RelationalTransitionSystem ρ σ l] (r : ρ) : σ → Prop where
   | init : ∀ (s : σ), sys.assumptions r → sys.init r s → reachable r s
   | step : ∀ (s s' : σ), reachable r s → sys.next r s s' → reachable r s'
 
 /-- Assumptions hold in all reachable states. -/
-theorem reachable_assumptions [sys : RelationalTransitionSystem ρ σ] (r : ρ) (s : σ) (h : reachable r s) : sys.assumptions r := by
+theorem reachable_assumptions [sys : RelationalTransitionSystem ρ σ l] (r : ρ) (s : σ) (h : reachable r s) : sys.assumptions r := by
   induction h with
   | init s has hinit => assumption
   | step s s' h2 hn ih => assumption
 
-theorem reachable_inclusion (sys sys' : RelationalTransitionSystem ρ σ)
+theorem reachable_inclusion (sys sys' : RelationalTransitionSystem ρ σ l)
   (hass_implies : ∀ (r : ρ), sys.assumptions r → sys'.assumptions r)
   (hinit_implies : ∀ (r : ρ) (st : σ), sys.init r st → sys'.init r st)
   (hnext_implies : ∀ (r : ρ) (st st' : σ), sys.next r st st' → sys'.next r st st') :
@@ -53,19 +59,105 @@ theorem reachable_inclusion (sys sys' : RelationalTransitionSystem ρ σ)
   | step s s' h2 hn ih => apply reachable.step ; apply ih ; apply hnext_implies ; assumption
 
 /-- The property holds in all reachable states. -/
-def isInvariant [sys : RelationalTransitionSystem ρ σ] (p : ρ → σ → Prop) : Prop := ∀ (r : ρ) (s : σ), reachable r s → p r s
+def isInvariant [sys : RelationalTransitionSystem ρ σ l] (p : ρ → σ → Prop) : Prop := ∀ (r : ρ) (s : σ), reachable r s → p r s
 
-theorem invariant_merge [sys : RelationalTransitionSystem ρ σ] (p q : ρ → σ → Prop) :
+theorem invariant_merge [sys : RelationalTransitionSystem ρ σ l] (p q : ρ → σ → Prop) :
   (isInvariant p ∧ isInvariant q) ↔ (isInvariant (fun r s => p r s ∧ q r s)) := by
   unfold isInvariant ; simp ; constructor
   next => intro ⟨ha, hb⟩ r s hh ; specialize ha _ _ hh ; specialize hb _ _ hh ; constructor <;> assumption
   next => intro h ; constructor <;> intro r s hh <;> specialize h _ _ hh <;> cases h <;> assumption
 
-theorem inductive_is_invariant [sys : RelationalTransitionSystem ρ σ] (p : ρ → σ → Prop) :
+theorem inductive_is_invariant [sys : RelationalTransitionSystem ρ σ l] (p : ρ → σ → Prop) :
   isInductive (sys := sys) p → isInvariant (sys := sys) p := by
   intro ⟨ha, hb⟩ r s₀ h
   induction h with
   | init s hass hinit => apply (ha _ _ hass hinit)
   | step s s' h2 hn ih => apply (hb r _ _ (reachable_assumptions r s h2) ih hn)
+
+theorem isInvariant_reachable [sys : RelationalTransitionSystem ρ σ l] (p : ρ → σ → Prop) :
+  isInvariant (sys := sys) p → ∀ (r : ρ) (s : σ), reachable r s → p r s := by
+  intro h r s hh
+  induction hh with
+  | init s hass hinit => aesop (add safe apply reachable.init)
+  | step s s' h2 hn ih => aesop (add safe apply reachable.step)
+
+structure Transition (ρ σ) [RelationalTransitionSystem ρ σ l] where
+  postState : σ
+  label : l
+
+abbrev StateTrace (ρ σ) [sys : RelationalTransitionSystem ρ σ l] := Array (Transition ρ σ)
+
+structure Trace (ρ σ) [sys : RelationalTransitionSystem ρ σ l] where
+  r₀ : ρ
+  s₀ : σ
+  tr : StateTrace ρ σ
+
+def StateTrace.isValidFrom [sys : RelationalTransitionSystem ρ σ l] (r : ρ) (s : σ) (ts : StateTrace ρ σ) : Prop :=
+  match _ : ts.toList with
+  | [] => True
+  | ⟨s', l⟩ :: ts' => sys.nextLab r s l s' ∧ isValidFrom r s' ts'.toArray
+termination_by ts.size
+decreasing_by
+  rename_i h; simp
+  have := congrArg List.length h
+  simp at this; omega
+
+def StateTrace.push [sys : RelationalTransitionSystem ρ σ l] (ts : StateTrace ρ σ) (s : σ) (l : l) : StateTrace ρ σ :=
+  Array.push ts ⟨s, l⟩
+
+def StateTrace.getLastD  [sys : RelationalTransitionSystem ρ σ l] (s : σ) (ts : StateTrace ρ σ) : σ :=
+  if let some ⟨s', _⟩ := ts.back? then s' else s
+
+def Trace.getLast [sys : RelationalTransitionSystem ρ σ l] (t : Trace ρ σ) : σ :=
+  t.tr.getLastD t.s₀
+
+def Trace.push [sys : RelationalTransitionSystem ρ σ l] (t : Trace ρ σ) (s : σ) (l : l) : Trace ρ σ :=
+  { t with tr := t.tr.push s l }
+
+@[simp]
+theorem StateTrace.getLastD_push [sys : RelationalTransitionSystem ρ σ l] (s : σ) (ts : StateTrace ρ σ) (s' : σ) (l : l) :
+  (ts.push s' l).getLastD s = s' := by
+  simp [getLastD, push]
+
+@[simp]
+theorem Trace.getLast_push [sys : RelationalTransitionSystem ρ σ l] (t : Trace ρ σ) (s : σ) (l : l) :
+  (t.push s l).getLast = s := by
+  simp [getLast, push]
+
+theorem StateTrace.push_isValidFrom [sys : RelationalTransitionSystem ρ σ l]
+  (r : ρ) (s : σ) (ts : StateTrace ρ σ) (s' : σ) (l : l) :
+  ts.isValidFrom r s ->
+  sys.nextLab r (ts.getLastD s) l s' ->
+  (ts.push s' l).isValidFrom r s := by
+  unhygienic fun_induction StateTrace.isValidFrom generalizing l s'
+  { cases ts_1 <;> simp at *
+    simp [*]; unfold StateTrace.isValidFrom; unfold StateTrace.push;
+    simp [Array.push, List.concat]
+    unfold StateTrace.isValidFrom; simp [getLastD] }
+  rename_i s
+  unfold isValidFrom; rw [h]; simp
+  unfold StateTrace.push; simp [Array.push]
+  rw [h]; simp [List.concat]
+  intro h' vl nx; constructor <;> try assumption
+  have : (push ts'.toArray s' l) = (ts' ++ [Transition.mk s' l]).toArray := by
+    rw [<-Array.toList_inj]
+    simp [push]
+  rw [<-this]; apply ih1; assumption
+  have : ts_1 = ts_1.toList.toArray := by simp
+  rw [this] at nx; revert nx
+  simp [h, getLastD, List.getLast?_cons]
+  cases ts'.getLast? <;> simp
+
+def Trace.isValid [sys : RelationalTransitionSystem ρ σ l] (t : Trace ρ σ) : Prop :=
+  sys.assumptions t.r₀ -> t.tr.isValidFrom t.r₀ t.s₀
+
+theorem Trace.push_isValid [sys : RelationalTransitionSystem ρ σ l] (t : Trace ρ σ) (s : σ) (l : l) :
+  t.isValid ->
+  sys.nextLab t.r₀ t.getLast l s ->
+  (t.push s l).isValid := by
+  cases t <;> simp [getLast, isValid, push]
+  intros; solve_by_elim [StateTrace.push_isValidFrom]
+
+
 
 end RelationalTransitionSystem
